steel/formats/spec/Zeta.Formats.LogEntry.fsti
@@ -1,0 +1,10 @@
+module Zeta.Formats.LogEntry
+
+module LP = LowParse.Spec.Base
+
+val parse_log_entry_kind: (k: LP.parser_kind { k.LP.parser_kind_subkind == Some LP.ParserStrong })
+
+val parse_log_entry (relate_payload: bool) : Tot (LP.parser parse_log_entry_kind (Zeta.Steel.LogEntry.Types.log_entry0 relate_payload))
+
+val serialize_log_entry (relate_payload: bool) : Tot (LP.serializer (parse_log_entry relate_payload))
+
