steel/formats/spec/Zeta.Formats.Synth.fsti
@@ -2,6 +2,34 @@ module Zeta.Formats.Synth
 
 module LPC = LowParse.Spec.Combinators
 
+val synth_key
+  (x: Zeta.Formats.Aux.Key.key)
+: Tot Zeta.Steel.LogEntry.Types.key
+
+val synth_key_recip
+  (x: Zeta.Steel.LogEntry.Types.key)
+: Tot Zeta.Formats.Aux.Key.key
+
+val synth_key_injective
+: squash (LPC.synth_injective synth_key)
+
+val synth_key_inverse
+: squash (LPC.synth_inverse synth_key synth_key_recip)
+
+val synth_mval_value
+  (x: Zeta.Formats.Aux.Mval_value.mval_value)
+: Tot Zeta.Steel.LogEntry.Types.mval_value
+
+val synth_mval_value_recip
+  (x: Zeta.Steel.LogEntry.Types.mval_value)
+: Tot Zeta.Formats.Aux.Mval_value.mval_value
+
+val synth_mval_value_injective
+: squash (LPC.synth_injective synth_mval_value)
+
+val synth_mval_value_inverse
+: squash (LPC.synth_inverse synth_mval_value synth_mval_value_recip)
+
 val synth_record
   (x: Zeta.Formats.Aux.Record.record)
 : Tot Zeta.Steel.LogEntry.Types.record
