steel/formats/spec/Zeta.Steel.LogEntry.Spec.fst
@@ -1,0 +1,3 @@
+module Zeta.Steel.LogEntry.Spec
+
+let spec_parser_log_entry = Zeta.Formats.LogEntry.parse_log_entry _
